AP/Util/Data/Trie/Raw.lean
@@ -4,13 +4,13 @@ namespace Trie
 
 open Std
 
-variable {α β : Type*} [ha₁ : DecidableEq α] [ha₂ : Hashable α]
-
 structure Raw (α β : Type*) [DecidableEq α] [Hashable α] where
   inner : Raw₀ α β
   wf : inner.WF
 
 namespace Raw
+
+variable {α β : Type*} [ha₁ : DecidableEq α] [ha₂ : Hashable α]
 
 set_option linter.unusedVariables false in
 def rec' {γ : Raw α β → Sort*}
@@ -20,8 +20,3 @@ def rec' {γ : Raw α β → Sort*}
 | .mk (Raw₀.mk val mp) wf => motive val mp wf # λ i t h₁ wf₁ => (mk t wf₁).rec' motive
 termination_by t => t.1.depthAux
 decreasing_by exact Raw₀.depthAux_le wf h₁
-
--- def Raw.depth : Raw α β → ℕ :=
---   Raw.rec' # λ val mp f => (mp.foldlWith sorry · 0) # by
---   intro acc i x h
---   exact max acc # 1 + f i x sorry
